EP+_Measure: - adjusted some of the initial definitions (some also renamed) - started structured proof of swap_decreases_measure Reductions: - added some inverted_pairs lemmas, - structured proof of adj_inv_pair_within_inverted_pair (renamed from adj_inv_exists_n) Executions: - added some trace_of_efrag lemmas

txn-data-consistency/EP+_Measure.thy
@@ -11,30 +11,34 @@ definition mover_type :: "'v ev list \<Rightarrow> nat \<Rightarrow> nat \<Right
    (if EVI tr i \<le> EVI tr k then Lm else Rm)
     else Out)"
 
-definition lmp_Lm_dist_left where
-  "lmp_Lm_dist_left tr \<equiv> let (j, k) = left_most_adj_pair ev_ects tr in
-    Sum {i - j | i. mover_type tr i j k = Lm}"
+definition left_movers :: "'v ev list \<Rightarrow> nat \<Rightarrow> nat \<Rightarrow> nat set" where
+  "left_movers tr j k \<equiv> {i. mover_type tr i j k = Lm}"
+
+abbreviation left_most_Lm where
+  "left_most_Lm tr j k \<equiv> Min (left_movers tr j k)"
 
 definition lmp_left_movers :: "'v ev list \<Rightarrow> nat set" where
   "lmp_left_movers tr \<equiv> let (j, k) = left_most_adj_pair ev_ects tr in
-    {i. mover_type tr i j k = Lm}"
+    left_movers tr j k"
 
-abbreviation left_most_Lm where
-  "left_most_Lm tr i j k \<equiv> j \<le> i \<and> Suc i \<le> k
-     \<and> (\<forall>i'. j \<le> i' \<and> i' \<le> i \<longrightarrow> mover_type tr i' j k = Rm)
-     \<and> mover_type tr (Suc i) j k = Lm"
+definition lmp_Lm_dist_left :: "'v ev list \<Rightarrow> nat" where
+  "lmp_Lm_dist_left tr \<equiv> let (j, k) = left_most_adj_pair ev_ects tr in
+    left_most_Lm tr j k - j"
 
-definition left_most_Lm_dist_left :: "'v ev list \<Rightarrow> nat" where
-  "left_most_Lm_dist_left tr \<equiv> let (j, k) = left_most_adj_pair ev_ects tr in
-    (THE i. left_most_Lm tr i j k) - j"
+(*
+definition lmp_Sum_Lm_dist_left where
+  "lmp_Sum_Lm_dist_left tr \<equiv> let (j, k) = left_most_adj_pair ev_ects tr in
+    Sum {i - j | i. mover_type tr i j k = Lm}"
 
 definition measure_R' :: "('v ev, ('v, 'm) global_conf_scheme) exec_frag rel" where
-  "measure_R' \<equiv> measures [card o inverted_pairs ev_ects o trace_of_efrag, lmp_Lm_dist_left o trace_of_efrag]"
+  "measure_R' \<equiv> measures [card o inverted_pairs ev_ects o trace_of_efrag, 
+                           lmp_Sum_Lm_dist_left o trace_of_efrag]"
+*)
 
 definition measure_R :: "('v ev, ('v, 'm) global_conf_scheme) exec_frag rel" where
   "measure_R \<equiv> measures [card o inverted_pairs ev_ects o trace_of_efrag,
                            card o lmp_left_movers o trace_of_efrag,
-                           left_most_Lm_dist_left o trace_of_efrag]" \<comment> \<open>Is this better?\<close>
+                           lmp_Lm_dist_left o trace_of_efrag]" \<comment> \<open>Is this better?\<close>
 
 lemma wf_measure_R: "wf measure_R"
   by (auto simp add: measure_R_def)
@@ -93,7 +97,7 @@ proof -
 qed
 
 
-subsection \<open>measure function lemmas\<close>
+subsection \<open>Measure function lemmas\<close>
 
 lemma i_Suci1:
   assumes
@@ -279,7 +283,7 @@ proof -
   done
 qed
 
-lemma swap_reduces_card:
+lemma swap_reduces_card_inverted_pairs:
   assumes
     \<open>adj_inv_pair f (l @ e2 # e1 # l') j k\<close>
     \<open>length l = i\<close>
@@ -620,28 +624,82 @@ lemma swap_mover_type:
         split: if_split_asm) sorry
   done
 
+
+term arg_min
+
+
 (* To chsp: this is the main lemma for proving the measure decreases. Currently I am stuck in the
   second case which uses swap_preserves_lmp(line 490) as its core lemma.*)
 lemma swap_decreases_measure: 
   assumes
     \<open>left_most_adj_pair ev_ects (trace_of_efrag ef) = (j, k)\<close>
-    \<open>adj_inv_pair ev_ects (trace_of_efrag ef) j k\<close>
-    \<open>j \<le> i \<and> Suc i \<le> k\<close>
+    \<open>adj_inv_pair ev_ects (trace_of_efrag ef) j k\<close>   (* there is some redundancy in assm(1-2) *)
+    \<open>j \<le> i\<close> \<open>Suc i \<le> k\<close>     (* remove conjunctions and existential quantifiers from premises *)
     \<open>k < length (ef_list ef)\<close>
-    \<open>left_most_Lm (trace_of_efrag ef) i j k\<close>
+    \<open>Suc i = left_most_Lm (trace_of_efrag ef) j k\<close>
     \<open>length efl = i\<close>
     \<open>valid_exec_frag tps ef\<close>
     \<open>ef = Exec_frag s0 (efl @ (s, e2, m) # (m, e1, s') # efl') sf\<close>
-  shows \<open>(Exec_frag s0 (efl @ (s, e1, w) # (w, e2, s') # efl') sf, ef) \<in> measure_R\<close>
+    \<open>ef' = Exec_frag s0 (efl @ (s, e1, w) # (w, e2, s') # efl') sf\<close>
+  shows \<open>(ef', ef) \<in> measure_R\<close> (* for all w? *)
   using assms
+
+  term "measures [card o inverted_pairs ev_ects o trace_of_efrag,
+                           card o lmp_left_movers o trace_of_efrag,
+                           lmp_Lm_dist_left o trace_of_efrag]"
+(*
+  This proof should be structured and proceed by case analysis:
+
+  case 1) j = i and Suc i = k, i.e., Suc j = k:
+     decreases "card o inverted_pairs ev_ects o trace_of_efrag"
+
+  case 2) j = i and Suc i < k:
+     preserves "card o inverted_pairs ev_ects o trace_of_efrag"
+     decreases "card o lmp_left_movers o trace_of_efrag"
+
+  case 3) j < i and Suc i \<le> k:
+     preserves "card o inverted_pairs ev_ects o trace_of_efrag"
+     preserves "card o lmp_left_movers o trace_of_efrag"
+     decreases "lmp_Lm_dist_left o trace_of_efrag"
+*)
+proof (cases "j = i")
+  case True
+  then show ?thesis 
+  proof (cases "Suc i = k")
+    case True
+    then have 
+      "card (inverted_pairs ev_ects (trace_of_efrag ef')) <
+       card (inverted_pairs ev_ects (trace_of_efrag ef))"
+    using \<open>j = i\<close> assms(1,2,5-)
+    by (auto simp add: trace_of_efrag_append_cons2 trace_of_efrag_length 
+             dest: swap_reduces_card_inverted_pairs)
+    then show ?thesis
+      by (simp add: measure_R_def)
+  next
+    case False
+    then have \<open>Suc i < k\<close> using \<open>Suc i \<le> k\<close> by simp
+    then show ?thesis using \<open>j = i\<close> assms(1,2,5-)
+
+      sorry
+  qed
+next
+  case False
+  then show ?thesis 
+
+    sorry
+qed
+
+
+
+(*
   apply (auto simp add: measure_R_def cons_form_to_index trace_of_decomposed_frag)
   subgoal \<comment> \<open>card inverted_pairs\<close>
     by (smt (verit) assms(4) exec_frag.sel(2) length_map lessI swap_preserves_card
-      swap_reduces_card trace_of_decomposed_frag trace_of_efrag_length)
+      swap_reduces_card_inverted_pairs trace_of_decomposed_frag trace_of_efrag_length)
   subgoal \<comment> \<open>card lmp_left_movers\<close> 
     apply (cases "i = j"; cases "Suc i = k")
     subgoal \<comment> \<open>i = j \<and> Suc i = k\<close>
-      by (smt (verit) assms(4) exec_frag.sel(2) length_map lessI swap_reduces_card
+      by (smt (verit) assms(4) exec_frag.sel(2) length_map lessI swap_reduces_card_inverted_pairs
           trace_of_decomposed_frag trace_of_efrag_length)
     subgoal \<comment> \<open>i = j \<and> Suc i \<noteq> k\<close> sorry
     subgoal \<comment> \<open>i \<noteq> j \<and> Suc i = k)\<close> sorry
@@ -649,9 +707,12 @@ lemma swap_decreases_measure:
       using swap_preserves_lmp[of ev_ects _ e2]
       apply (simp add: lmp_left_movers_def pair_after_swap_def swap_i_Suci_def)
       using swap_mover_type[of j _ k e2] card_image[OF inj_on_swap_i_Suci]
-      by auto.
+      by auto
+    done
   subgoal \<comment> \<open>dist left_most Lm in lmp from left\<close>
   sorry
   done
+*)
+
 
 end
